WIP equivalence relation

vera/VerilogEquivalenceCorrectness.v
@@ -44,59 +44,6 @@ Local Open Scope monad_scope.
 
 Import SigTNotations.
 
-Definition execution_defined_match_on C e1 e2 :=
-  e1 ={ C }= e2 /\ RegisterState.defined_value_for C e1.
-
-Notation "rs1 =!!{ P }!!= rs2" :=
-  (execution_defined_match_on P rs1 rs2)
-  (at level 80) : type_scope.
-
-Notation "rs1 =!!( vars )!!= rs2" :=
-  (rs1 =!!{fun var => In var vars}!!= rs2)
-  (at level 80) : type_scope.
-
-Lemma defined_match_on_iff C e1 e2 :
-  e1 =!!{ C }!!= e2 <->
-  forall var, C var -> exists bv, e1 var = Some (XBV.from_bv bv) /\ e2 var = Some (XBV.from_bv bv).
-Proof.
-  unfold execution_defined_match_on, "_ ={ _ }= _", RegisterState.defined_value_for.
-  split. 
-  - intros [Hmatch Hdefined] var HC. insterU Hmatch. insterU Hdefined.
-    rewrite <- Hmatch. crush.
-  - intro H. split.
-    + intros var HC. insterU H. destruct H as [? [? ?]]. crush.
-    + intros var HC. insterU H. destruct H as [? [? ?]]. crush.
-Qed.
-
-Lemma execution_defined_match_on_trans C e1 e2 e3:
-  e1 =!!{ C }!!= e2 ->
-  e2 =!!{ C }!!= e3 ->
-  e1 =!!{ C }!!= e3.
-Proof.
-  unfold "_ =!!{ _ }!!= _".
-  intros [] [].
-  split.
-  - now transitivity e2.
-  - eassumption.
-Qed.
-
-Lemma execution_defined_match_on_sym C e1 e2:
-  e1 =!!{ C }!!= e2 ->
-  e2 =!!{ C }!!= e1.
-Proof.
-  unfold "_ =!!{ _ }!!= _".
-  intros [].
-  split.
-  - now symmetry.
-  - now rewrite <- H.
-Qed.
-
-Add Parametric Relation (C : Verilog.variable -> Prop) :
-  RegisterState.t (execution_defined_match_on C)
-  symmetry proved by (execution_defined_match_on_sym C)
-  transitivity proved by (execution_defined_match_on_trans C)
-  as execution_defiened_match_on_rel.
-
 Ltac decompose_all_records :=
   repeat match goal with
          | [ H : _ |- _ ] => progress (decompose record H); clear H
@@ -938,85 +885,10 @@ Proof.
   assumption.
 Qed.
 
-Definition equivalent_behaviour (v1 v2 : Verilog.vmodule) : Prop :=
-  forall e1 e2,
-    valid_execution v1 e1 ->
-    valid_execution v2 e2 ->
-    e1 =!!(Verilog.module_inputs v1)!!= e2 ->
-    e1 =!!(Verilog.module_outputs v1)!!= e2.
-
-Lemma equivalent_behaviour_trans v1 v2 v3:
-  equivalent_behaviour v1 v2 ->
-  equivalent_behaviour v2 v3 ->
-  equivalent_behaviour v1 v3.
-Proof.
-  unfold equivalent_behaviour.
-  intros H12 H23 e1 e3 Hvalid1 Hvalid3 Heq_inputs13.
-  assert (exists e2, (valid_execution v2 e2 /\ (e1 =!!( Verilog.module_inputs v1 )!!= e2))) by admit.
-  destruct H as [e2 [Hvalid2 Heq_inputs12]].
-  specialize (H12 e1 e2). insterU H12.
-  transitivity e2; [eassumption|].
-  replace (Verilog.module_inputs v2) with (Verilog.module_inputs v1) in * by admit.
-  replace (Verilog.module_outputs v2) with (Verilog.module_outputs v1) in * by admit.
-  specialize (H23 e2 e3).
-  eapply H23; eauto.
-  transitivity e1; (idtac + symmetry); eassumption.
-Admitted.
-
-Lemma equivalent_behaviour_sym v1 v2:
-  equivalent_behaviour v1 v2 ->
-  equivalent_behaviour v2 v1.
-Proof.
-  unfold equivalent_behaviour.
-  intros H e1 e2 Hvalid1 Hvalid2 Heq_inputs.
-  replace (Verilog.module_outputs v2) with (Verilog.module_outputs v1) by admit.
-  symmetry. eapply H; try eassumption.
-  replace (Verilog.module_inputs v1) with (Verilog.module_inputs v2) by admit.
-  symmetry.
-  assumption. 
-Admitted.
-
-Lemma equivalent_behaviour_refl v: equivalent_behaviour v v.
-Proof.
-  unfold equivalent_behaviour, valid_execution.
-  intros.
-Admitted.
-
-Add Parametric Relation :
-  Verilog.vmodule equivalent_behaviour
-  reflexivity proved by equivalent_behaviour_refl
-  symmetry proved by equivalent_behaviour_sym
-  transitivity proved by equivalent_behaviour_trans
-  as equivalent_behaviour_rel.
-
-Record equivalent v1 v2:=
-  MkEquivalent
-    {
-      equiv_inputs : Verilog.module_inputs v1 = Verilog.module_inputs v2;
-      equiv_outputs : Verilog.module_outputs v1 = Verilog.module_outputs v2;
-      equiv_behaviour : equivalent_behaviour v1 v2
-    }.
-
-(* Lemma equivalent_trans v1 v2 v3:
- *   equivalent v1 v2 ->
- *   equivalent v2 v3 ->
- *   equivalent v1 v3.
- * Proof. Admitted.
- * 
- * Lemma equivalent_sym v1 v2:
- *   equivalent v1 v2 ->
- *   equivalent v2 v1.
- * Proof. Admitted.
- * 
- * Lemma equivalent_refl v: equivalent v v.
- * Proof. Admitted.
- * 
- * Add Parametric Relation :
- *   Verilog.vmodule equivalent
- *   reflexivity proved by equivalent_refl
- *   symmetry proved by equivalent_sym
- *   transitivity proved by equivalent_trans
- *   as equivalent_rel. *)
+Definition module_valid v :
+  forall initial,
+    (forall var, In var (Verilog.module_inputs v) -> exists val, initial var = Some val) ->
+    exists final, run_vmodule v initial = Some final.
 
 Lemma no_counterexample_equivalent_iff v1 v2 :
   (forall e1 e2, ~ counterexample_execution v1 e1 v2 e2) <-> (equivalent_behaviour v1 v2).
